embedding/theories/EnvSubst.v
@@ -5,6 +5,7 @@ From Coq Require Import Morphisms.
 From Coq Require Import ssrbool.
 From Coq Require Import PeanoNat.
 
+From ConCert.Utils Require Import Extras.
 From ConCert.Embedding Require Import EvalE.
 From ConCert.Embedding Require Import Ast.
 From ConCert.Embedding Require Import CustomTactics.
@@ -36,7 +37,7 @@ Module NamelessSubst.
         tyApp ty1' ty2'
       | tyVar nm => ty
       | tyRel i => if Nat.leb k i then
-                    from_option (lookup_ty ρ (i-k)) (tyRel i) else tyRel i
+                    with_default (tyRel i) (lookup_ty ρ (i-k)) else tyRel i
       | tyArr ty1 ty2 =>
         let ty2' := subst_env_i_ty k ρ ty2 in
         let ty1' := subst_env_i_ty k ρ ty1 in
@@ -48,7 +49,7 @@ Module NamelessSubst.
   Fixpoint subst_env_i_aux (k : nat) (ρ : env expr) (e : expr) : expr :=
     match e with
     | eRel i => if Nat.leb k i then
-                 from_option (lookup_i ρ (i-k)) (eRel i) else eRel i
+                 with_default (eRel i) (lookup_i ρ (i-k)) else eRel i
     | eVar nm  => eVar nm
     | eLambda nm ty b => eLambda nm (subst_env_i_ty k ρ ty) (subst_env_i_aux (1+k) ρ b)
     | eTyLam nm b => eTyLam nm (subst_env_i_aux (1+k) ρ b)
@@ -149,7 +150,7 @@ Module NamelessSubst.
            simpl in *. unfold inst_env_i,subst_env_i in *. simpl in *.
            rewrite <- H2. replace (n2 - 0) with n2 by lia.
            apply lookup_i_of_val_env in H1.
-           now eapply from_option_indep.
+           now eapply with_default_indep.
   Qed.
 
 End NamelessSubst.
