examples/bat/BATCommon.v
@@ -17,10 +17,10 @@ From Coq Require Import List.
 From Coq Require Import Permutation.
 From Coq Require Import ZArith.
 From ConCert.Utils Require Import Automation.
+From ConCert.Utils Require Import Extras.
 From ConCert.Utils Require Import RecordUpdate.
 From ConCert.Execution Require Import Blockchain.
 From ConCert.Execution Require Import Containers.
-From ConCert.Execution Require Import Extras.
 From ConCert.Execution Require Import Serializable.
 From ConCert.Examples.EIP20 Require EIP20Token.
 Import RecordSetNotations.
