examples/bat/BATTests.v
@@ -1,8 +1,8 @@
 From QuickChick Require Import QuickChick.
 Import QcNotation.
+From ConCert.Utils Require Import Extras.
 From ConCert.Execution Require Import Blockchain.
 From ConCert.Execution Require Import BoundedN.
-From ConCert.Execution Require Import Extras.
 From ConCert.Execution Require Import Containers.
 From ConCert.Execution Require Import LocalBlockchain.
 From ConCert.Execution Require Import Serializable.
