examples/bat/BAT_AltFix.v
@@ -14,11 +14,11 @@ From Coq Require Import Lia.
 From Coq Require Import Morphisms.
 From Coq Require Import ZArith.
 From ConCert.Utils Require Import Automation.
+From ConCert.Utils Require Import Extras.
 From ConCert.Utils Require Import RecordUpdate.
 From ConCert.Execution Require Import Blockchain.
 From ConCert.Execution Require Import BuildUtils.
 From ConCert.Execution Require Import Containers.
-From ConCert.Execution Require Import Extras.
 From ConCert.Execution Require Import Monads.
 From ConCert.Execution Require Import Serializable.
 From ConCert.Execution Require Import Common.
