examples/boardroomVoting/BoardroomMath.v
@@ -10,7 +10,7 @@ From Bignums Require Import BigZ.
 
 From ConCert.Examples.BoardroomVoting Require Import Egcd.
 From ConCert.Examples.BoardroomVoting Require Import Euler.
-From ConCert.Execution Require Import Extras.
+From ConCert.Utils Require Import Extras.
 Import ListNotations.
 
 Local Open Scope Z.
