examples/boardroomVoting/BoardroomVotingZ.v
@@ -3,10 +3,10 @@ From Coq Require Import ZArith.
 From Coq Require Import Znumtheory.
 From Coq Require Import Permutation.
 From Coq Require Import Psatz.
+From ConCert.Utils Require Import Extras.
 From ConCert.Utils Require Import RecordUpdate.
 From ConCert.Execution Require Import Blockchain.
 From ConCert.Execution Require Import Containers.
-From ConCert.Execution Require Import Extras.
 From ConCert.Execution Require Import Monads.
 From ConCert.Execution Require Import Serializable.
 From ConCert.Execution Require Import Common. Import AddressMap.
