examples/congress/Congress.v
@@ -9,11 +9,11 @@ From Coq Require Import Psatz.
 From Coq Require Import List.
 From ConCert.Execution Require Import Blockchain.
 From ConCert.Execution Require Import Containers.
-From ConCert.Execution Require Import Extras.
 From ConCert.Execution Require Import Monads.
 From ConCert.Execution Require Import ResultMonad.
 From ConCert.Execution Require Import Serializable.
 From ConCert.Utils Require Import Automation.
+From ConCert.Utils Require Import Extras.
 From ConCert.Utils Require Import RecordUpdate.
 
 Import ListNotations.
