examples/congress/Congress_Buggy.v
@@ -11,10 +11,10 @@ From Coq Require Import List.
 From ConCert.Execution Require Import Blockchain.
 From ConCert.Execution Require Import BoundedN.
 From ConCert.Execution Require Import Containers.
-From ConCert.Execution Require Import Extras.
 From ConCert.Execution Require Import Monads.
 From ConCert.Execution Require Import ResultMonad.
 From ConCert.Execution Require Import Serializable.
+From ConCert.Utils Require Import Extras.
 From ConCert.Utils Require Import RecordUpdate.
 
 Import ListNotations.
