examples/congress/tests/Congress_BuggyTests.v
@@ -11,13 +11,13 @@ From ConCert.Execution Require Import BoundedN.
 From ConCert.Execution Require Import Containers.
 From ConCert.Execution Require Import ResultMonad.
 From ConCert.Execution Require Import Monads.
-From ConCert.Execution Require Import Extras.
 From ConCert.Execution.QCTests Require Import TestUtils.
 From ConCert.Execution.QCTests Require Import TraceGens.
 From ConCert.Execution.QCTests Require Import ChainPrinters.
 From ConCert.Examples.Congress Require Import Congress_Buggy.
 From ConCert.Examples.Congress Require Import Congress_BuggyGens.
 From ConCert.Examples.Congress Require Import Congress_BuggyPrinters.
+From ConCert.Utils Require Import Extras.
 From ConCert.Utils Require Import RecordUpdate.
 Close Scope monad_scope.
 
