examples/counter/Counter.v
@@ -5,7 +5,7 @@ From Coq Require Import ZArith.
 From Coq Require Import List.
 From Coq Require Import Basics.
 From ConCert.Utils Require Import Automation.
-From ConCert.Execution Require Import Extras.
+From ConCert.Utils Require Import Extras.
 From ConCert.Execution Require Import Serializable.
 From ConCert.Execution Require Import Blockchain.
 
