examples/crowdfunding/ExecFrameworkIntegration.v
@@ -16,8 +16,8 @@ From Coq Require Import ssrbool.
 From Coq Require Import Program.Tactics.
 
 From ConCert.Utils Require Import Automation.
+From ConCert.Utils Require Import Extras.
 From ConCert.Execution Require Import Blockchain.
-From ConCert.Execution Require Import Extras.
 From ConCert.Execution Require Import ResultMonad.
 
 Import ListNotations.
