examples/dexter/DexterTests.v
@@ -4,12 +4,12 @@ From ConCert.Execution Require Import Containers.
 From ConCert.Execution Require Import BoundedN.
 From ConCert.Execution Require Import Monads.
 From ConCert.Execution Require Import ResultMonad.
-From ConCert.Execution Require Import Extras.
 From ConCert.Execution.QCTests Require Import TestUtils.
 From ConCert.Examples.FA2 Require Import FA2Token.
 From ConCert.Examples.FA2 Require Import FA2Interface.
 From ConCert.Examples.Dexter Require Import Dexter.
 From ConCert.Examples.Dexter Require Import DexterGens.
+From ConCert.Utils Require Import Extras.
 From ConCert.Utils Require Import RecordUpdate.
 
 From QuickChick Require Import QuickChick.
