examples/dexter2/Dexter2CPMM.v
@@ -13,9 +13,9 @@
 *)
 
 From ConCert.Utils Require Import Automation.
+From ConCert.Utils Require Import Extras.
 From ConCert.Utils Require Import RecordUpdate.
 From ConCert.Execution Require Import Blockchain.
-From ConCert.Execution Require Import Extras.
 From ConCert.Execution Require Import Monads.
 From ConCert.Execution Require Import Serializable.
 From ConCert.Execution Require Import InterContractCommunication.
