examples/eip20/EIP20Token.v
@@ -11,11 +11,11 @@ From Coq Require Import Lia.
 From Coq Require Import Permutation.
 From ConCert.Execution Require Import Containers.
 From ConCert.Execution Require Import Monads.
-From ConCert.Execution Require Import Extras.
 From ConCert.Execution Require Import Serializable.
 From ConCert.Execution Require Import Blockchain.
 From ConCert.Execution Require Import Common.
 From ConCert.Utils Require Import Automation.
+From ConCert.Utils Require Import Extras.
 From ConCert.Utils Require Import RecordUpdate.
 
 Import ListNotations.
