examples/eip20/EIP20TokenTests.v
@@ -1,10 +1,10 @@
 Global Set Warnings "-extraction-logical-axiom".
 
 From QuickChick Require Import QuickChick. Import QcNotation.
+From ConCert.Utils Require Import Extras.
 From ConCert.Execution Require Import Blockchain.
 From ConCert.Execution Require Import BoundedN.
 From ConCert.Execution Require Import Containers.
-From ConCert.Execution Require Import Extras.
 From ConCert.Execution Require Import LocalBlockchain.
 From ConCert.Execution Require Import Serializable.
 From ConCert.Execution Require Import ResultMonad.
