examples/fa2/FA2Token.v
@@ -1,10 +1,10 @@
 From Coq Require Import List.
 From Coq Require Import Program.Basics.
 From Coq Require Import ZArith.
+From ConCert.Utils Require Import Extras.
 From ConCert.Utils Require Import RecordUpdate.
 From ConCert.Execution Require Import Blockchain.
 From ConCert.Execution Require Import Containers.
-From ConCert.Execution Require Import Extras.
 From ConCert.Execution Require Import Monads.
 From ConCert.Execution Require Import Serializable.
 From ConCert.Execution Require Import Common.
