execution/theories/Blockchain.v
@@ -64,11 +64,11 @@ From Coq Require Import Psatz.
 From Coq Require Import Permutation.
 From Coq Require Import Morphisms.
 From ConCert.Execution Require Import ChainedList.
-From ConCert.Execution Require Import Extras.
 From ConCert.Execution Require Import Monads.
 From ConCert.Execution Require Import ResultMonad.
 From ConCert.Execution Require Import Serializable.
 From ConCert.Utils Require Import Automation.
+From ConCert.Utils Require Import Extras.
 From ConCert.Utils Require Import RecordUpdate.
 
 Import ListNotations.
