execution/theories/LocalBlockchain.v
@@ -8,11 +8,11 @@ From ConCert.Execution Require Import Blockchain.
 From ConCert.Execution Require Import BoundedN.
 From ConCert.Execution Require Import ChainedList.
 From ConCert.Execution Require Import Containers.
-From ConCert.Execution Require Import Extras.
 From ConCert.Execution Require Import Monads.
 From ConCert.Execution Require Import ResultMonad.
 From ConCert.Execution Require Import Serializable.
 From ConCert.Utils Require Import Automation.
+From ConCert.Utils Require Import Extras.
 From ConCert.Utils Require Import RecordUpdate.
 From Coq Require Import ZArith.
 From Coq Require Import Permutation.
